viper-total-heaps/PredicateRel.thy
@@ -3,6 +3,313 @@ theory PredicateRel
 begin
 
 
+subsection \<open>Inhale\<close>
+
+definition inhale_pred_normal_premise
+  where "inhale_pred_normal_premise ctxt StateCons pred_id ty_args e_args e_p vs p \<omega> \<omega>' \<equiv>
+       vals_well_typed (absval_interp_total ctxt) vs ty_args \<and>
+       red_pure_exps_total ctxt (Some \<omega>) e_args \<omega> (Some vs) \<and>
+       ctxt, Some \<omega> \<turnstile> \<langle>e_p; \<omega>\<rangle> [\<Down>]\<^sub>t Val (VPerm p) \<and>
+       p \<ge> 0 \<and>
+       (let W' = inhale_perm_single_pred ctxt StateCons \<omega> (pred_id, vs) (Some (Abs_preal p)) in
+         (W' \<noteq> {} \<and> \<omega>' \<in> W'))"
+
+
+lemma inhale_predicate_acc_rel:
+  assumes WfSubexp: "exprs_wf_rel (\<lambda>\<omega>def \<omega> ns. R \<omega> ns \<and> \<omega>def = \<omega> \<and> Q (Atomic (AccPredicate pred_id e_args (PureExp e_p))) \<omega>) 
+                       ctxt_vpr StateCons P ctxt (e_args @ [e_p]) \<gamma> \<gamma>2"
+      and PosPermRel: "\<And>p. rel_general R (R' p)
+                         (\<lambda> \<omega> \<omega>'. \<omega> = \<omega>' \<and> (ctxt_vpr, Some \<omega> \<turnstile> \<langle>e_p;\<omega>\<rangle> [\<Down>]\<^sub>t (Val (VPerm p)) \<and> p \<ge> 0))
+                         (\<lambda> \<omega>. (ctxt_vpr, Some \<omega> \<turnstile> \<langle>e_p;\<omega>\<rangle> [\<Down>]\<^sub>t (Val (VPerm p)) \<and> p < 0))
+                         P ctxt \<gamma>2 \<gamma>3"
+      and UpdInhRel: "\<And>vs p. rel_general (R' p) R \<comment>\<open>Here, the simulation needs to revert back to R\<close>
+                         (inhale_pred_normal_premise ctxt_vpr StateCons pred_id tys_args e_args e_p vs p)
+                         (\<lambda> \<omega>. False) P ctxt \<gamma>3 \<gamma>'" 
+    shows "inhale_rel R Q ctxt_vpr StateCons P ctxt (Atomic (AccPredicate pred_id e_args (PureExp e_p))) \<gamma> \<gamma>'"
+  sorry
+
+
+lemma add_to_lpm_nonzero_total_full__mp:
+  shows "get_mp_total_full (add_to_lpm_nonzero_total_full nm lp p \<phi>) = (get_mp_total_full nm)(lp := get_mp_total_full nm lp + Rep_posreal p)"
+  sorry
+
+
+lemma inhale_rel_pred_acc_upd_rel:
+  assumes
+    StateRel: "\<And> \<omega> ns. R \<omega> ns \<Longrightarrow>
+                         state_rel_def_same Pr StateCons TyRep Tr
+                           (AuxPred(temp_perm \<mapsto> pred_eq (RealV p))) ctxt \<omega> ns" and
+              "temp_perm \<notin> dom AuxPred" and
+
+    WfTyRep: "wf_ty_repr_bpl TyRep" and
+    MaskVarDefSame: "mask_var_def Tr = mask_var Tr" and
+    TyInterp: "type_interp ctxt = vbpl_absval_ty TyRep" and
+
+    NullConst: "const_repr Tr CNull = nullConst" and
+    MaskVar: "m_bpl = mask_var Tr" and
+    PredLocBpl: "e_ploc_bpl = FunExp ''P'' [] [e_arg_bpl]" and
+
+    MaskUpdateWf: "mask_update_wf TyRep ctxt mask_upd_bpl" and
+    MaskReadWf: "mask_read_wf TyRep ctxt mask_read_bpl" and
+
+    NewPermBpl: "new_perm = (mask_read_bpl (Var m_bpl) (Var nullConst) e_ploc_bpl
+                                  [TConSingle ''PredicateType_P'', TPrim TBool]) \<guillemotleft>Add\<guillemotright> (Var temp_perm)" and
+    MaskUpdateBpl: "m_upd_bpl = mask_upd_bpl (Var m_bpl) (Var nullConst) e_ploc_bpl new_perm
+                                  [TConSingle ''PredicateType_P'', TPrim TBool]" and
+
+    ArgRel: "exp_rel_vpr_bpl
+                (state_rel Pr StateCons TyRep Tr (AuxPred(temp_perm \<mapsto> pred_eq (RealV p))) ctxt)
+                ctxt_vpr ctxt e_arg_vpr e_arg_bpl" and
+
+    PredFunInterp: "fun_interp ctxt ''P'' = Some (lift_fun_bpl (vbpl_absval_ty TyRep) (0, [TConSingle (TRefId TyRep)], TCon (TFieldId TyRep) [TCon ''PredicateType_P'' [], TPrim TBool]) predicate_loc_P)" and
+    PredName: "pred_id = ''P''" and
+    PredLookup: "ViperLang.predicates (program_total ctxt_vpr) pred_id = Some pdecl" and
+    PredTyArgsLookup: "predicate_decl.args pdecl = ty_args" and
+    PredTyArgs: "ty_args = [TRef]" and
+    AbsInterpEq: "absval_interp_total ctxt_vpr = domain_type TyRep" and
+    ProgEq: "program_total ctxt_vpr = Pr"
+
+  shows "rel_general R
+           (state_rel_def_same Pr StateCons TyRep Tr AuxPred ctxt)
+           (\<lambda> \<omega> \<omega>'. inhale_pred_normal_premise ctxt_vpr StateCons pred_id ty_args [e_arg_vpr] e_p_vpr vs p \<omega> \<omega>')
+           (\<lambda> \<omega>. False) P ctxt
+           (BigBlock name ((Assign m_bpl m_upd_bpl) # cs) str tr, cont)
+           (BigBlock name cs str tr, cont)"
+
+  apply (rule rel_intro)
+   prefer 2
+   apply blast
+proof -
+  fix \<omega> ns \<omega>'
+  assume "R \<omega> ns"
+     and *: "inhale_pred_normal_premise ctxt_vpr StateCons pred_id ty_args [e_arg_vpr] e_p_vpr vs p \<omega> \<omega>'"
+
+  hence InitRel: "state_rel_def_same Pr StateCons TyRep Tr
+                                     (AuxPred(temp_perm \<mapsto> pred_eq (RealV p))) ctxt \<omega> ns"
+    using StateRel
+    by blast
+
+  hence InitRel': "state_rel_def_same Pr StateCons TyRep Tr AuxPred ctxt \<omega> ns"
+    apply (rule state_rel_aux_pred_remove[where ?AuxPred="AuxPred(temp_perm \<mapsto> pred_eq (RealV p))" and ?AuxPred'=AuxPred])
+    by (simp add: assms(2) map_le_def)
+
+  from * have "length vs = 1"
+    by (metis One_nat_def add.right_neutral add_Suc_right inhale_pred_normal_premise_def list.size(3) list.size(4) red_pure_exps_total_Some_lengthD)
+  then obtain arg where "vs = [arg]"
+    by (metis One_nat_def Suc_le_eq impossible_Cons length_greater_0_conv list.exhaust list.size(3) n_not_Suc_n)
+  with * have 1: "inhale_pred_normal_premise ctxt_vpr StateCons pred_id ty_args [e_arg_vpr] e_p_vpr [arg] p \<omega> \<omega>'"
+    by fast
+
+  let ?ploc = "(pred_id,[arg])"
+
+  obtain \<phi>_inh where \<omega>':
+    "(p > 0 \<longrightarrow> consistent_external_wrt_ploc ctxt_vpr \<phi>_inh ?ploc (Abs_preal p)) \<and>
+     get_hh_total \<phi>_inh = get_hh_total_full \<omega> \<and>
+     \<omega>' = (if p = 0 then \<omega> else add_to_lpm_nonzero_total_full \<omega> ?ploc (Abs_posreal (Abs_preal p)) (get_nm_total \<phi>_inh)) \<and>
+     StateCons \<omega>'"
+    using 1[simplified inhale_pred_normal_premise_def inhale_perm_single_pred_def Let_def]
+    by (smt (verit) mem_Collect_eq option_fold.simps(1) positive_real_preal pperm_pnone_pgt zero_preal.abs_eq)
+
+  hence mh_same: "get_mh_total_full \<omega> = get_mh_total_full \<omega>'" and
+        mp_rel: "get_mp_total_full \<omega>' = (get_mp_total_full \<omega>)( ?ploc := get_mp_total_full \<omega> ?ploc + Abs_preal p )"
+     apply simp
+    apply (cases "p = 0")
+    using \<omega>' zero_preal_def
+     apply force
+    using \<omega>'[THEN conjunct2, THEN conjunct2, THEN conjunct1]
+    apply (simp del: add_to_lpm_nonzero_total_full.simps get_mp_total_full.simps)
+    using add_to_lpm_nonzero_total_full__mp
+    by (metis 1 all_pos inhale_pred_normal_premise_def mem_Collect_eq order_le_less positive_real_preal posreal_to_preal(8))
+
+  have \<omega>'_extcons: "consistent_state_rel_opt (state_rel_opt Tr) \<Longrightarrow>
+    consistent_external (total_context.make Pr (\<lambda>_. None) (domain_type TyRep)) (get_total_full \<omega>')"
+    apply (cases "p = 0")
+     apply (metis InitRel' \<omega>' state_rel_consistent)
+  proof -
+    assume "consistent_state_rel_opt (state_rel_opt Tr)"
+      and "p \<noteq> 0"
+    have "consistent_external (total_context.make Pr (\<lambda>_. None) (domain_type TyRep)) (get_total_full \<omega>)"
+      using InitRel' \<open>consistent_state_rel_opt (state_rel_opt Tr)\<close> state_rel_consistent
+      by blast
+    have "\<omega>' = add_to_lpm_nonzero_total_full \<omega> ?ploc (Abs_posreal (Abs_preal p)) (get_nm_total \<phi>_inh)"
+      by (simp add: \<omega>' \<open>p \<noteq> 0\<close>)
+    have "consistent_external_wrt_ploc ctxt_vpr \<phi>_inh ?ploc (Abs_preal p)"
+      using 1 \<omega>' \<open>p \<noteq> 0\<close> inhale_pred_normal_premise_def
+      by force
+    hence 2: "consistent_external_wrt_ploc ctxt_vpr
+                \<lparr> get_hh_total = get_hh_total_full \<omega>, get_nm_total = get_nm_total \<phi>_inh \<rparr>
+                ?ploc (Abs_preal p)"
+      by (metis (full_types) \<omega>' old.unit.exhaust total_state.surjective)
+    show ?thesis
+      unfolding \<open>\<omega>' = _\<close>
+      apply (rule extcons_preserved_by_add_to_lpm_nonzero)
+        apply fact
+       apply (rule extcons_fun_interp_irrelevant[of ctxt_vpr])
+         apply (simp add: total_context.defs)
+         apply fact
+        apply (simp add: total_context.defs AbsInterpEq)
+       apply fact
+      by (metis * \<open>p \<noteq> 0\<close> inhale_pred_normal_premise_def order_neq_le_trans positive_real_preal pperm_pnone_pgt)
+  qed
+
+  obtain mb where
+    LookupMask: "lookup_var (var_context ctxt) ns (mask_var Tr) = Some (AbsV (AMask mb))" and
+    LookupMaskTy: "lookup_var_ty (var_context ctxt) (mask_var Tr) = Some (TConSingle (TMaskId TyRep))" and
+    MaskRel: "mask_rel Pr (field_translation Tr) (get_mh_total_full \<omega>) (get_mp_total_full \<omega>) mb"
+    using state_rel_obtain_mask[OF StateRel[OF \<open>R \<omega> ns\<close>]]
+    by blast
+
+  \<comment> \<open>Construct the value of the new permission from the Viper state.\<close>
+  let ?np = "Rep_preal (get_mp_total_full \<omega> (pred_id,[arg])) + p"
+
+  have LookupTempPerm: "lookup_var (var_context ctxt) ns temp_perm = Some (RealV p)"
+    using state_rel_aux_pred_sat_lookup_2[OF StateRel[OF \<open>R \<omega> ns\<close>]]
+    unfolding pred_eq_def
+    by (metis (full_types) fun_upd_same)
+
+  have null_eval: "red_expr_bpl ctxt (Var nullConst) ns (AbsV (ARef Null))"
+    apply (rule red_expr_red_exprs.RedVar)
+    by (metis NullConst StateRel \<open>R \<omega> ns\<close> boogie_const_rel_lookup boogie_const_val.simps(3) state_rel_boogie_const_rel)
+
+  have e_arg_eval: "red_expr_bpl ctxt e_arg_bpl ns (val_rel_vpr_bpl arg)"
+    using ArgRel[simplified exp_rel_vpr_bpl_def exp_rel_vb_single_def]
+    by (metis 1 InitRel inhale_pred_normal_premise_def list.simps(3) nth_Cons_0 red_exp_list_normal_elim)
+
+  have e_arg_type: "get_type (absval_interp_total ctxt_vpr) arg = TRef"
+    using 1[simplified inhale_pred_normal_premise_def vals_well_typed_def PredTyArgs]
+    by blast
+  then obtain arg_bpl where arg_bpl: "val_rel_vpr_bpl arg = AbsV (ARef arg_bpl)"
+    by (metis has_type_get_type has_type_simps(8) val_rel_vpr_bpl.simps(3))
+
+  have ploc_eval: "red_expr_bpl ctxt e_ploc_bpl ns (AbsV (AField (PredSnapshotField (pred_id, [arg]))))"
+    apply (simp add: PredLocBpl)
+    apply (rule red_expr_red_exprs.RedFunOp)
+    using PredFunInterp
+      apply blast
+     apply (rule red_expr_red_exprs.RedExpListCons)
+    using e_arg_eval
+      apply blast
+     apply (rule red_expr_red_exprs.RedExpListNil)
+    apply (simp add: arg_bpl)
+    using arg_bpl PredName e_arg_type has_type_get_type
+    apply (simp add: lift_fun_bpl_def)
+    by force
+
+  have new_perm_eval: "red_expr_bpl ctxt new_perm ns (LitV (LReal ?np))"
+    apply (simp add: NewPermBpl)
+    apply (rule red_expr_red_exprs.RedBinOp[where ?v1.0="LitV (LReal (Rep_preal (get_mp_total_full \<omega> (pred_id,[arg]))))" and ?v2.0="LitV (LReal p)"])
+      apply (rule mask_read_wf_apply[OF MaskReadWf, where ?m=mb and ?r=Null and ?f="PredSnapshotField (pred_id,[arg])"])
+          apply (metis MaskRel mask_rel_def)
+         apply (simp add: LookupMask MaskVar red_expr_red_exprs.RedVar)
+        apply (simp add: null_eval)
+       apply (simp add: ploc_eval)
+      apply force
+     apply (fastforce intro: RedVar LookupTempPerm)
+    by simp
+
+  \<comment> \<open>Construct the new Boogie heap.\<close>
+  let ?mb' = "mb( (Null, PredSnapshotField (pred_id,[arg])) := ?np )"
+
+  have m_upd_bpl_red: "red_expr_bpl ctxt m_upd_bpl ns (AbsV (AMask ?mb'))"
+    apply (subst \<open>m_upd_bpl = _\<close>)
+    apply (rule mask_update_wf_apply[OF MaskUpdateWf])
+        apply (simp add: LookupMask MaskVar red_expr_red_exprs.RedVar)
+       apply (simp add: null_eval)
+      apply (simp add: ploc_eval)
+    using new_perm_eval
+     apply blast
+    by simp
+
+  have "valid_heap_mask (get_mh_total_full \<omega>)"
+    using InitRel state_rel_wf_mask_simple by blast
+
+  have Disj: "disjoint_list [ {heap_var Tr, heap_var_def Tr},
+                              {mask_var Tr, mask_var_def Tr},
+                              ran (var_translation Tr),
+                              ran (field_translation Tr),
+                              range (const_repr Tr), dom AuxPred]"
+    using InitRel' state_rel_disjoint
+    by blast
+
+  show "\<exists>ns'. red_ast_bpl P ctxt
+                ((BigBlock name (Assign m_bpl m_upd_bpl # cs) str tr, cont), Normal ns)
+                ((BigBlock name cs str tr, cont), Normal ns') \<and>
+              state_rel_def_same Pr StateCons TyRep Tr AuxPred ctxt \<omega>' ns'"
+    apply (rule exI, intro conjI)
+     apply (rule red_ast_bpl_one_simple_cmd)
+     apply (rule RedAssign[where ?ty="TConSingle (TMaskId TyRep)" and ?v="AbsV (AMask ?mb')"])
+    using MaskVar StateRel \<open>R \<omega> ns\<close> state_rel_obtain_mask
+       apply blast
+      apply (simp add: TyInterp)
+    using m_upd_bpl_red
+     apply blast
+    apply (simp only: state_rel_def)
+    apply (simp only: state_rel0_def, intro conjI)
+    using state_rel_wf_mask_simple[OF InitRel] \<omega>'
+                    apply (simp, simp)
+    using \<omega>'_extcons \<omega>'
+                  apply blast
+                 apply (simp add: TyInterp)
+                apply (rule store_rel_stable[where ?\<omega>=\<omega> and ?ns=ns])
+    using InitRel state_rel_store_rel
+                  apply blast
+                 apply (metis 1 inhale_perm_single_pred_store_same inhale_pred_normal_premise_def)
+                apply (metis InitRel MaskVar state_rel_disj_mask_store update_var_other)
+               apply (simp add: Disj)
+              apply (simp, simp, simp)
+           defer defer defer defer
+           apply (metis InitRel MaskVar field_rel_stable mask_var_disjoint state_rel_field_rel state_rel_state_rel0 update_var_other)
+          apply (metis InitRel MaskVar boogie_const_rel_stable mask_var_disjoint state_rel_boogie_const_rel state_rel_state_rel0 update_var_other)
+         defer
+         apply (metis (no_types, lifting) InitRel' MaskVar aux_vars_pred_sat_def domI mask_var_disjoint state_rel_aux_pred_sat_lookup state_rel_state_rel0 update_var_other)
+  proof -
+    let ?ns' = "update_var (var_context ctxt) ns m_bpl
+                  (AbsV (AMask (mb((Null, PredSnapshotField (pred_id, [arg])) :=
+                                   Rep_preal (get_mp_total_full \<omega> (pred_id, [arg])) + p))))"
+
+    \<comment> \<open>Prove \<^const>\<open>heap_var_rel\<close>\<close>
+    show HeapRel: "heap_var_rel Pr (var_context ctxt) TyRep (field_translation Tr) (heap_var Tr) \<omega>' ?ns'"
+      apply (rule heap_var_rel_stable[OF state_rel0_heap_var_rel[OF InitRel[simplified state_rel_def]]])
+       apply (metis 1 inhale_perm_single_pred_heap_same inhale_pred_normal_premise_def)
+      by (metis InitRel MaskVar mask_var_disjoint state_rel_state_rel0 update_var_other)
+
+    \<comment> \<open>Prove \<^const>\<open>mask_var_rel\<close>\<close>
+    show MaskRel: "mask_var_rel Pr (var_context ctxt) TyRep (field_translation Tr) (mask_var Tr) \<omega>' ?ns'"
+      apply (unfold mask_var_rel_def)
+      apply (rule exI[of _ ?mb'])
+      apply (intro conjI)
+        apply (simp add: MaskVar)
+      using LookupMaskTy
+       apply blast
+      apply (unfold mask_rel_def)
+      apply (intro conjI)
+      using MaskRel[simplified mask_rel_def] mh_same
+         apply auto[1]
+        apply (simp add: MaskRel[simplified mask_rel_def])
+      using MaskRel[simplified mask_rel_def]
+       apply (smt (verit, best) 1 MaskRel[simplified mask_rel_def] fun_upd_apply inhale_pred_normal_premise_def is_bounded_field_bpl.simps(1) prod.sel(2))
+      apply (subst \<open>get_mp_total_full \<omega>' = _\<close>)
+      by (metis (no_types, lifting) 1 Abs_preal_inverse MaskRel[simplified mask_rel_def] fun_upd_apply inhale_pred_normal_premise_def mem_Collect_eq plus_preal.rep_eq prod.inject vb_field.simps(2))
+
+    show "heap_var_rel Pr (var_context ctxt) TyRep (field_translation Tr) (heap_var_def Tr) \<omega>' ?ns'"
+      apply (rule heap_var_rel_stable[OF state_rel_heap_var_def_rel[OF InitRel]])
+       apply (metis 1 inhale_perm_single_pred_heap_same inhale_pred_normal_premise_def)
+      by (metis InitRel MaskVar mask_var_disjoint state_rel_state_rel0 update_var_other)
+
+    show MaskRel: "mask_var_rel Pr (var_context ctxt) TyRep (field_translation Tr) (mask_var_def Tr) \<omega>' ?ns'"
+      apply (subst MaskVarDefSame)
+      using MaskRel
+      by blast
+
+    show "state_well_typed (type_interp ctxt) (var_context ctxt) [] ?ns'"
+      apply (rule state_well_typed_upd_2)
+      using InitRel state_rel_state_well_typed
+       apply blast
+      by (simp add: TyInterp LookupMaskTy MaskVar)
+  qed
+qed
+
+
 subsection \<open>External Consistent State \<Longrightarrow> Inhaled State\<close>
 
 lemma get_mp_0_implies_fnm_None:
@@ -860,251 +1167,6 @@ proof -
     using WfCons
      apply simp
     by fact
-qed
-
-
-subsection \<open>Inhale\<close>
-
-lemma inhale_rel_pred_acc_upd_rel:
-  assumes
-    StateRel: "\<And> \<omega> ns. R \<omega> ns \<Longrightarrow>
-                         state_rel_def_same Pr StateCons TyRep Tr
-                           (AuxPred(temp_perm \<mapsto> pred_eq (RealV p))) ctxt \<omega> ns" and
-              "temp_perm \<notin> dom AuxPred" and
-
-    WfTyRep: "wf_ty_repr_bpl TyRep" and
-    MaskVarDefSame: "mask_var_def Tr = mask_var Tr" and
-    TyInterp: "type_interp ctxt = vbpl_absval_ty TyRep" and
-
-    NullConst: "const_repr Tr CNull = nullConst" and
-    MaskVar: "m_bpl = mask_var Tr" and
-    PredLocBpl: "e_ploc_bpl = FunExp ''P'' [] [e_arg_bpl]" and
-
-    MaskUpdateWf: "mask_update_wf TyRep ctxt mask_upd_bpl" and
-    MaskReadWf: "mask_read_wf TyRep ctxt mask_read_bpl" and
-
-    NewPermBpl: "new_perm = (mask_read_bpl (Var m_bpl) (Var nullConst) e_ploc_bpl
-                                  [TConSingle ''PredicateType_P'', TPrim TBool]) \<guillemotleft>Add\<guillemotright> (Var temp_perm)" and
-    MaskUpdateBpl: "m_upd_bpl = mask_upd_bpl (Var m_bpl) (Var nullConst) e_ploc_bpl new_perm
-                                  [TConSingle ''PredicateType_P'', TPrim TBool]" and
-
-    ArgRel: "exp_rel_vpr_bpl
-                (state_rel Pr StateCons TyRep Tr (AuxPred(temp_perm \<mapsto> pred_eq (RealV p))) ctxt)
-                ctxt_vpr ctxt e_arg_vpr e_arg_bpl" and
-
-    PredFunInterp: "fun_interp ctxt ''P'' = Some (lift_fun_bpl (vbpl_absval_ty TyRep) (0, [TConSingle (TRefId TyRep)], TCon (TFieldId TyRep) [TCon ''PredicateType_P'' [], TPrim TBool]) predicate_loc_P)" and
-    PredName: "pred_id = ''P''" and
-    PredLookup: "ViperLang.predicates (program_total ctxt_vpr) pred_id = Some pdecl" and
-    PredTyArgsLookup: "predicate_decl.args pdecl = ty_args" and
-    PredTyArgs: "ty_args = [TRef]"
-
-  shows "rel_general R
-           (state_rel_def_same Pr StateCons TyRep Tr AuxPred ctxt)
-           (\<lambda> \<omega> \<omega>'. inhale_pred_normal_premise ctxt_vpr StateCons pred_id ty_args [e_arg_vpr] e_p_vpr vs p \<omega> \<omega>')
-           (\<lambda> \<omega>. False) P ctxt
-           (BigBlock name ((Assign m_bpl m_upd_bpl) # cs) str tr, cont)
-           (BigBlock name cs str tr, cont)"
-
-  apply (rule rel_intro)
-   prefer 2
-   apply blast
-proof -
-  fix \<omega> ns \<omega>'
-  assume "R \<omega> ns"
-     and *: "inhale_pred_normal_premise ctxt_vpr StateCons pred_id ty_args [e_arg_vpr] e_p_vpr vs p \<omega> \<omega>'"
-
-  hence InitRel: "state_rel_def_same Pr StateCons TyRep Tr
-                                     (AuxPred(temp_perm \<mapsto> pred_eq (RealV p))) ctxt \<omega> ns"
-    using StateRel
-    by blast
-
-  hence InitRel': "state_rel_def_same Pr StateCons TyRep Tr AuxPred ctxt \<omega> ns"
-    apply (rule state_rel_aux_pred_remove[where ?AuxPred="AuxPred(temp_perm \<mapsto> pred_eq (RealV p))" and ?AuxPred'=AuxPred])
-    by (simp add: assms(2) map_le_def)
-
-  from * have "length vs = 1"
-    by (metis One_nat_def add.right_neutral add_Suc_right inhale_pred_normal_premise_def list.size(3) list.size(4) red_pure_exps_total_Some_lengthD)
-  then obtain arg where "vs = [arg]"
-    by (metis One_nat_def Suc_le_eq impossible_Cons length_greater_0_conv list.exhaust list.size(3) n_not_Suc_n)
-  with * have 1: "inhale_pred_normal_premise ctxt_vpr StateCons pred_id ty_args [e_arg_vpr] e_p_vpr [arg] p \<omega> \<omega>'"
-    by fast
-
-  let ?ploc = "(pred_id,[arg])"
-
-  obtain \<phi>_inh where \<omega>':
-    "(p > 0 \<longrightarrow> consistent_external_wrt_ploc ctxt_vpr \<phi>_inh ?ploc (Abs_preal p)) \<and>
-     get_hh_total \<phi>_inh = get_hh_total_full \<omega> \<and>
-     \<omega>' = (if p = 0 then \<omega> else add_to_lpm_nonzero_total_full \<omega> ?ploc (Abs_posreal (Abs_preal p)) (get_nm_total \<phi>_inh)) \<and>
-     StateCons \<omega>'"
-    using 1[simplified inhale_pred_normal_premise_def inhale_perm_single_pred_def]
-    by (smt (verit, ccfv_threshold) mem_Collect_eq option_fold.simps(1) positive_real_preal pperm_pnone_pgt zero_preal.abs_eq)
-
-  hence mh_same: "get_mh_total_full \<omega> = get_mh_total_full \<omega>'" and
-         mp_rel: "get_mp_total_full \<omega>' = (get_mp_total_full \<omega>)( ?ploc := get_mp_total_full \<omega> ?ploc + Abs_preal p )"
-     apply simp
-    apply (cases "p = 0")
-    using \<omega>' zero_preal_def
-     apply force
-    sorry
-
-  have \<omega>'_extcons: "consistent_external ctxt_vpr (get_total_full \<omega>')"
-    sorry
-
-  obtain mb where
-    LookupMask: "lookup_var (var_context ctxt) ns (mask_var Tr) = Some (AbsV (AMask mb))" and
-    LookupMaskTy: "lookup_var_ty (var_context ctxt) (mask_var Tr) = Some (TConSingle (TMaskId TyRep))" and
-    MaskRel: "mask_rel Pr (field_translation Tr) (get_mh_total_full \<omega>) (get_mp_total_full \<omega>) mb"
-    using state_rel_obtain_mask[OF StateRel[OF \<open>R \<omega> ns\<close>]]
-    by blast
-
-  \<comment> \<open>Construct the value of the new permission from the Viper state.\<close>
-  let ?np = "Rep_preal (get_mp_total_full \<omega> (pred_id,[arg])) + p"
-
-  have LookupTempPerm: "lookup_var (var_context ctxt) ns temp_perm = Some (RealV p)"
-    using state_rel_aux_pred_sat_lookup_2[OF StateRel[OF \<open>R \<omega> ns\<close>]]
-    unfolding pred_eq_def
-    by (metis (full_types) fun_upd_same)
-
-  have null_eval: "red_expr_bpl ctxt (Var nullConst) ns (AbsV (ARef Null))"
-    apply (rule red_expr_red_exprs.RedVar)
-    by (metis NullConst StateRel \<open>R \<omega> ns\<close> boogie_const_rel_lookup boogie_const_val.simps(3) state_rel_boogie_const_rel)
-
-  have e_arg_eval: "red_expr_bpl ctxt e_arg_bpl ns (val_rel_vpr_bpl arg)"
-    using ArgRel[simplified exp_rel_vpr_bpl_def exp_rel_vb_single_def]
-    by (metis 1 InitRel inhale_pred_normal_premise_def list.simps(3) nth_Cons_0 red_exp_list_normal_elim)
-
-  have e_arg_type: "get_type (absval_interp_total ctxt_vpr) arg = TRef"
-    using 1[simplified inhale_pred_normal_premise_def vals_well_typed_def PredTyArgs]
-    by blast
-  then obtain arg_bpl where arg_bpl: "val_rel_vpr_bpl arg = AbsV (ARef arg_bpl)"
-    by (metis has_type_get_type has_type_simps(8) val_rel_vpr_bpl.simps(3))
-
-  have ploc_eval: "red_expr_bpl ctxt e_ploc_bpl ns (AbsV (AField (PredSnapshotField (pred_id, [arg]))))"
-    apply (simp add: PredLocBpl)
-    apply (rule red_expr_red_exprs.RedFunOp)
-    using PredFunInterp
-      apply blast
-     apply (rule red_expr_red_exprs.RedExpListCons)
-    using e_arg_eval
-      apply blast
-     apply (rule red_expr_red_exprs.RedExpListNil)
-    apply (simp add: arg_bpl)
-    using arg_bpl PredName e_arg_type has_type_get_type
-    apply (simp add: lift_fun_bpl_def)
-    by force
-
-  have new_perm_eval: "red_expr_bpl ctxt new_perm ns (LitV (LReal ?np))"
-    apply (simp add: NewPermBpl)
-    apply (rule red_expr_red_exprs.RedBinOp[where ?v1.0="LitV (LReal (Rep_preal (get_mp_total_full \<omega> (pred_id,[arg]))))" and ?v2.0="LitV (LReal p)"])
-      apply (rule mask_read_wf_apply[OF MaskReadWf, where ?m=mb and ?r=Null and ?f="PredSnapshotField (pred_id,[arg])"])
-          apply (metis MaskRel mask_rel_def)
-         apply (simp add: LookupMask MaskVar red_expr_red_exprs.RedVar)
-        apply (simp add: null_eval)
-       apply (simp add: ploc_eval)
-      apply force
-     apply (fastforce intro: RedVar LookupTempPerm)
-    by simp
-
-  \<comment> \<open>Construct the new Boogie heap.\<close>
-  let ?mb' = "mb( (Null, PredSnapshotField (pred_id,[arg])) := ?np )"
-
-  have m_upd_bpl_red: "red_expr_bpl ctxt m_upd_bpl ns (AbsV (AMask ?mb'))"
-    apply (subst \<open>m_upd_bpl = _\<close>)
-    apply (rule mask_update_wf_apply[OF MaskUpdateWf])
-        apply (simp add: LookupMask MaskVar red_expr_red_exprs.RedVar)
-       apply (simp add: null_eval)
-      apply (simp add: ploc_eval)
-    using new_perm_eval
-     apply blast
-    by simp
-
-  have "valid_heap_mask (get_mh_total_full \<omega>)"
-    using InitRel state_rel_wf_mask_simple by blast
-
-  have Disj: "disjoint_list [ {heap_var Tr, heap_var_def Tr},
-                              {mask_var Tr, mask_var_def Tr},
-                              ran (var_translation Tr),
-                              ran (field_translation Tr),
-                              range (const_repr Tr), dom AuxPred]"
-    using InitRel' state_rel_disjoint
-    by blast
-
-  show "\<exists>ns'. red_ast_bpl P ctxt
-                ((BigBlock name (Assign m_bpl m_upd_bpl # cs) str tr, cont), Normal ns)
-                ((BigBlock name cs str tr, cont), Normal ns') \<and>
-              state_rel_def_same Pr StateCons TyRep Tr AuxPred ctxt \<omega>' ns'"
-    apply (rule exI, intro conjI)
-     apply (rule red_ast_bpl_one_simple_cmd)
-     apply (rule RedAssign[where ?ty="TConSingle (TMaskId TyRep)" and ?v="AbsV (AMask ?mb')"])
-    using MaskVar StateRel \<open>R \<omega> ns\<close> state_rel_obtain_mask
-       apply blast
-      apply (simp add: TyInterp)
-    using m_upd_bpl_red
-     apply blast
-    apply (simp only: state_rel_def)
-    apply (simp only: state_rel0_def, intro conjI)
-    using state_rel_wf_mask_simple[OF InitRel] \<omega>'
-                    apply (simp, simp)
-    using \<omega>' \<omega>'_extcons
-    subgoal sorry
-                 apply (simp add: TyInterp)
-                apply (rule store_rel_stable[where ?\<omega>=\<omega> and ?ns=ns])
-    using InitRel state_rel_store_rel
-                  apply blast
-                 apply (metis 1 inhale_perm_single_pred_store_same inhale_pred_normal_premise_def)
-                apply (metis InitRel MaskVar state_rel_disj_mask_store update_var_other)
-               apply (simp add: Disj)
-              apply (simp, simp, simp)
-           defer defer defer defer
-           apply (metis InitRel MaskVar field_rel_stable mask_var_disjoint state_rel_field_rel state_rel_state_rel0 update_var_other)
-          apply (metis InitRel MaskVar boogie_const_rel_stable mask_var_disjoint state_rel_boogie_const_rel state_rel_state_rel0 update_var_other)
-         defer
-         apply (metis (no_types, lifting) InitRel' MaskVar aux_vars_pred_sat_def domI mask_var_disjoint state_rel_aux_pred_sat_lookup state_rel_state_rel0 update_var_other)
-  proof -
-    let ?ns' = "update_var (var_context ctxt) ns m_bpl
-                  (AbsV (AMask (mb((Null, PredSnapshotField (pred_id, [arg])) :=
-                                   Rep_preal (get_mp_total_full \<omega> (pred_id, [arg])) + p))))"
-
-    \<comment> \<open>Prove \<^const>\<open>heap_var_rel\<close>\<close>
-    show HeapRel: "heap_var_rel Pr (var_context ctxt) TyRep (field_translation Tr) (heap_var Tr) \<omega>' ?ns'"
-      apply (rule heap_var_rel_stable[OF state_rel0_heap_var_rel[OF InitRel[simplified state_rel_def]]])
-       apply (metis 1 inhale_perm_single_pred_heap_same inhale_pred_normal_premise_def)
-      by (metis InitRel MaskVar mask_var_disjoint state_rel_state_rel0 update_var_other)
-
-    \<comment> \<open>Prove \<^const>\<open>mask_var_rel\<close>\<close>
-    show MaskRel: "mask_var_rel Pr (var_context ctxt) TyRep (field_translation Tr) (mask_var Tr) \<omega>' ?ns'"
-      apply (unfold mask_var_rel_def)
-      apply (rule exI[of _ ?mb'])
-      apply (intro conjI)
-        apply (simp add: MaskVar)
-      using LookupMaskTy
-       apply blast
-      apply (unfold mask_rel_def)
-      apply (intro conjI)
-      using MaskRel[simplified mask_rel_def] mh_same
-         apply auto[1]
-        apply (simp add: MaskRel[simplified mask_rel_def])
-      using MaskRel[simplified mask_rel_def]
-       apply (smt (verit, best) 1 MaskRel[simplified mask_rel_def] fun_upd_apply inhale_pred_normal_premise_def is_bounded_field_bpl.simps(1) prod.sel(2))
-      apply (subst \<open>get_mp_total_full \<omega>' = _\<close>)
-      by (metis (no_types, lifting) 1 Abs_preal_inverse MaskRel[simplified mask_rel_def] fun_upd_apply inhale_pred_normal_premise_def mem_Collect_eq plus_preal.rep_eq prod.inject vb_field.simps(2))
-
-    show "heap_var_rel Pr (var_context ctxt) TyRep (field_translation Tr) (heap_var_def Tr) \<omega>' ?ns'"
-      apply (rule heap_var_rel_stable[OF state_rel_heap_var_def_rel[OF InitRel]])
-       apply (metis 1 inhale_perm_single_pred_heap_same inhale_pred_normal_premise_def)
-      by (metis InitRel MaskVar mask_var_disjoint state_rel_state_rel0 update_var_other)
-
-    show MaskRel: "mask_var_rel Pr (var_context ctxt) TyRep (field_translation Tr) (mask_var_def Tr) \<omega>' ?ns'"
-      apply (subst MaskVarDefSame)
-      using MaskRel
-      by blast
-
-    show "state_well_typed (type_interp ctxt) (var_context ctxt) [] ?ns'"
-      apply (rule state_well_typed_upd_2)
-      using InitRel state_rel_state_well_typed
-       apply blast
-      by (simp add: TyInterp LookupMaskTy MaskVar)
-  qed
 qed
 
 
