tests/20250226_152528_try_proof/method_proof_foo/end_to_end_proof_foo.thy
@@ -26,6 +26,15 @@ apply ((unfold ctxt_wf_def))
 by (simp add: ctxt_bpl_def global_data_end_to_end.fun_interp_vpr_bpl_inst_wf)
 
 
+lemma CtxtWfPred:
+  shows "ctxt_wf_pred global_data_end_to_end.ctxt_vpr"
+  sorry
+
+lemma CtxtPredSelfFraming:
+  shows "ctxt_pred_self_framing global_data_end_to_end.ctxt_vpr"
+  sorry
+
+
 lemmas bound_lemmas = list_all_ran_map_of[OF relational_proof_foo.var_relation_list_1_bound] list_all_ran_map_of[OF field_rel_bound] const_repr_basic_bound_2
 
 
@@ -44,8 +53,8 @@ by ((force simp: relational_proof_foo.tr_vpr_bpl_0_def relational_proof_foo.var_
 
 lemma method_partial_proof : 
 assumes "(proc_is_correct (type_interp_bpl (absval_interp_total global_data_end_to_end.ctxt_vpr)) global_data.fdecls global_data.constants_vdecls global_data.unique_consts global_data.globals_vdecls global_data.axioms foo_before_ast_to_cfg_prog.ast_proc (Ast.proc_body_satisfies_spec::(((('a) vbpl_absval), ast) proc_body_satisfies_spec_ty)))"
-shows "(vpr_method_correct_total_partial (global_data_end_to_end.ctxt_vpr::(('a) total_context)) (\<lambda> _.True) method_decls.foo_decl)"
-apply ((rule end_to_end_vpr_method_correct_partial[where ?ctxt = ctxt_bpl, OF assms true_mono_prop_downward_ord wf_ty_repr_basic wf_total_consistency_trivial]))
+shows "(vpr_method_correct_total_partial (global_data_end_to_end.ctxt_vpr::(('a) total_context)) consistent_internal_total_full method_decls.foo_decl)"
+apply ((rule end_to_end_vpr_method_correct_partial[where ?ctxt = ctxt_bpl, OF assms mono_prop_downward_ord_consistent_internal_total_full wf_ty_repr_basic wf_total_consistency_internal[OF CtxtWfPred CtxtPredSelfFraming]]))
 apply ((simp add: ty_repr_basic_def))
 apply ((simp only: global_data_end_to_end.program_total_eq))
 apply ((rule method_decls.foo_lookup_lemma[simplified HOL.sym[OF global_data_vpr.methods_vpr_prog]]))
@@ -71,6 +80,8 @@ apply ((rule ctxt_wf))
 apply ((simp add: global_data_end_to_end.fun_interp_wf ctxt_bpl_def))
 apply ((simp add: global_data_end_to_end.program_total_eq))
 apply ((simp add: ctxt_bpl_def))
+apply (rule CtxtWfPred)
+apply (rule CtxtPredSelfFraming)
 apply ((simp add: relational_proof_foo.tr_vpr_bpl_0_def default_state_rel_options_def))
 apply (((rule exI))+)
 apply ((intro conjI))
